new/golang/theory/test.v
@@ -1,0 +1,38 @@
+From New.golang.theory Require Export postlifting.
+
+Section test.
+Context `{sem: ffi_semantics} `{!ffi_interp ffi} `{!heapGS Σ} {core_sem : go.CoreSemantics}.
+
+Definition someStructType : go.type :=
+  go.StructType [(go.FieldDecl "a"%go (go.PointerType (go.Named "uint64"%go [])))].
+
+Lemma wp_test  :
+  {{{ True }}}
+  GoEquals someStructType (StructV {[ "a"%go := #null ]}, StructV {[ "a"%go := #null ]})%V
+  {{{ RET #true; True }}}.
+Proof.
+  iIntros "% _ HΦ".
+
+  (* TODO: abstract into lemma *)
+  iApply (wp_GoInstruction [] (GoEquals someStructType)).
+  { intros. repeat econstructor. }
+  iNext; iIntros "* %Hstep"; inv Hstep; inv Hpure.
+  iIntros "? $ !>". simpl.
+
+  (* precondition/typeclass *)
+  assert (go.is_comparable someStructType) as Hcomp.
+  { rewrite go.is_comparable_struct. repeat constructor. apply into_val_comparable. }
+  rewrite Hcomp.
+
+  rewrite go._go_eq_struct. simpl.
+  wp_pures.
+  wp_apply wp_StructFieldGet_untyped. (* TODO: use struct field get instance *)
+  { rewrite lookup_singleton //. }
+  iIntros "_".
+  wp_apply wp_StructFieldGet_untyped.
+  { rewrite lookup_singleton //. }
+  iIntros "_".
+  wp_pures. by iApply "HΦ".
+Qed.
+
+End test.
